Factor out proof caching library

src/program_proof/examples/replicated_block_proof.v
@@ -80,36 +80,35 @@ Section goose.
   Proof.
     iIntros (? Φ Φc) "(Hinv&HP) HΦ"; iNamed "Hinv".
     iDeexHyp "Hbackup".
-    iAssert (□ ∀ b0, int.val addr d↦ σ ∗
-                     int.val (word.add addr 1) d↦ b0 ∗
-                     P σ -∗ rblock_cinv addr σ ∗ P σ)%I
-            as "#Hcrash".
-    { iIntros "!>" (b) "(Hb0&Hb1&HP)".
+    wpc_call.
+    { iFrame.
+      iExists _; iFrame. }
+    iCache with "Hprimary Hbackup HP HΦ".
+    { crash_case.
       iFrame.
       iExists _; iFrame. }
-    Ltac prove_crash1 :=
-      iApply ("Hcrash" with "[$]").
-    wpc_call; first by prove_crash1.
     wpc_apply (wpc_Read with "Hprimary").
     iSplit; [ | iNext ].
     { iIntros "Hprimary".
-      crash_case; prove_crash1. }
+      iFromCache. }
     iIntros (s) "(Hprimary&Hb)".
     iDestruct (is_slice_to_small with "Hb") as "Hb".
-    wpc_pures; first by prove_crash1.
-    wpc_apply (wpc_Write with "[Hbackup Hb]").
-    { iExists _; iFrame. }
+    wpc_pures.
+    wpc_apply (wpc_Write' with "[$Hbackup $Hb]").
     iSplit; [ | iNext ].
-    { iIntros "Hpost".
-      iDestruct "Hpost" as (b') "Hbackup".
-      crash_case; prove_crash1. }
+    { iIntros "[Hbackup|Hbackup]"; try iFromCache.
+      crash_case.
+      iFrame.
+      iExists _; iFrame. }
     iIntros "(Hbackup&_)".
+    iCache with "HP HΦ Hprimary Hbackup".
+    { crash_case; iFrame.
+      iExists _; iFrame. }
 
     (* allocate lock *)
-    wpc_pures; first by prove_crash1.
+    wpc_pures.
     wpc_bind (lock.new _).
     wpc_frame "HP Hprimary Hbackup HΦ". (* ie, everything *)
-    { crash_case; prove_crash1. }
     wp_apply wp_new_free_lock.
     iIntros (γ m_ref) "Hfree_lock".
     iNamed 1.
@@ -162,12 +161,6 @@ Section goose.
       iApply "HΦ"; auto.
   Qed.
 
-  Ltac wpc_bind_seq :=
-    lazymatch goal with
-    | [ |- envs_entails _ (wpc _ _ _ _ (App (Lam _ ?e2) ?e1) _ _) ] =>
-      wpc_bind e1
-    end.
-
   Theorem wpc_RepBlock__Read (Q: Block → iProp Σ) (Qc: iProp Σ) {k E2} {k' γ l} addr (primary: bool) :
     (S k < k')%nat →
     {{{ "Hrb" ∷ is_rblock γ k' l addr ∗
@@ -178,23 +171,25 @@ Section goose.
   Proof.
     iIntros (? Φ Φc) "Hpre HΦ"; iNamed "Hpre".
     iNamed "Hrb".
-    Ltac prove_crash1 ::=
-      crash_case; by iRight in "Hfupd".
-    wpc_call; first by prove_crash1.
-    wpc_bind_seq; wpc_frame "HΦ Hfupd"; first by prove_crash1.
+    wpc_call.
+    { by iRight in "Hfupd". }
+    iCache with "HΦ Hfupd".
+    { crash_case;
+        by iRight in "Hfupd". }
+    wpc_bind_seq; wpc_frame "HΦ Hfupd".
     wp_loadField.
     wp_apply (crash_lock.acquire_spec with "Hlock"); auto.
     iIntros "Hlkd"; iNamed 1.
     iDestruct "Hlkd" as (γlk) "His_locked".
-    wpc_pures; first by prove_crash1.
-    wpc_bind (RepBlock__readAddr _ _); wpc_frame "HΦ Hfupd"; first by prove_crash1.
+    wpc_pures.
+    wpc_bind (RepBlock__readAddr _ _); wpc_frame "HΦ Hfupd".
     wp_apply (wp_RepBlock__readAddr with "addr").
     iIntros (addr' Haddr'_eq).
     iNamed 1.
 
     wpc_bind_seq.
     iApply (use_crash_locked with "His_locked"); auto.
-    iSplit; first by prove_crash1.
+    iSplit; first by iFromCache.
     iNamed 1.
     iAssert (int.val addr' d↦ σ ∗
                    (int.val addr' d↦ σ -∗ rblock_linv addr σ))%I
@@ -234,108 +229,6 @@ Section goose.
     iApply "HΦ"; iFrame.
   Admitted.
 
-  Record cache {PROP:bi} (R: PROP) :=
-    Cache { cache_prop :> env PROP;
-            (* TODO: make this a string pattern *)
-            cache_names: list ident; }.
-
-  Arguments Cache {PROP}.
-  Arguments cache_names {PROP R} c.
-  Arguments cache_prop {PROP R} c.
-
-  Definition cached_def {R} (c: cache R): iProp Σ :=
-    □ ([∗] c -∗ R).
-  Definition cached_aux : seal (@cached_def). by eexists. Qed.
-  Definition cached := unseal cached_aux.
-  Definition cached_eq : @cached = @cached_def := seal_eq cached_aux.
-  Arguments cached {R} c.
-
-  Ltac unseal := rewrite cached_eq /cached_def.
-
-  Global Instance cached_Persistent : Persistent (@cached R c).
-  Proof. unseal; apply _. Qed.
-
-  Theorem tac_cached_use {Δ: envs (iPropI Σ)} i {R} (c: cache R) :
-    envs_lookup i Δ = Some (true, cached c) →
-    match envs_split base.Left c.(cache_names) Δ with
-    | Some (Γs, _) => Γs.(env_spatial) = c.(cache_prop)
-    | None => False
-    end →
-    envs_entails Δ R.
-  Proof.
-    rewrite cached_eq.
-    iIntros (Hlookup Hsubenv).
-    destruct_with_eqn (envs_split base.Left c.(cache_names) Δ); [ | contradiction ].
-    destruct p as [Γs Γ'].
-    rewrite envs_entails_eq.
-    iIntros "HΔ".
-    iDestruct (envs_lookup_intuitionistic_sound _ _ _ Hlookup with "HΔ") as
-        "[#Hcache HΔ]".
-    iDestruct (envs_split_sound with "HΔ") as "[HΔ1 HΔ2]"; eauto.
-    iDestruct (envs_clear_spatial_sound with "HΔ1") as "(HΔ'&HΔs)".
-    iApply "Hcache".
-    rewrite -Hsubenv.
-    iAssumption.
-  Qed.
-
-  Theorem cached_make R (c: cache R) :
-    □ (env_to_named_prop c -∗ R) -∗
-    cached c.
-  Proof.
-    unseal.
-    iIntros "#HR !>".
-    rewrite env_to_named_prop_unname.
-    rewrite env_to_prop_sound.
-    auto.
-  Qed.
-
-  Ltac iCache_go P Hs pat :=
-  let Hs := words Hs in
-  let Hs := eval vm_compute in (INamed <$> Hs) in
-  let Δ := iGetCtx in
-  let js := reduction.pm_eval (envs_split base.Left Hs Δ) in
-  match js with
-  | Some (?Δ, _) => let Γs := (eval cbv [env_spatial] in Δ.(env_spatial)) in
-                    iAssert (cached (Cache P Γs Hs)) as pat;
-                    [ iApply cached_make; iModIntro;
-                      cbv [env_to_named_prop env_to_named_prop_go cache_prop];
-                      iNamed 1
-                    | ]
-  | None => fail 1 "hypotheses not found"
-  end.
-
-  Tactic Notation "iCache" "with" constr(Hs) :=
-    lazymatch goal with
-    | [ |- envs_entails _ (wpc _ _ _ _ _ _ ?Φc) ] =>
-         iCache_go Φc Hs "#?"
-    end.
-
-  Ltac iFromCache :=
-    lazymatch goal with
-    | [ |- envs_entails (Envs ?Γp _ _) ?P ] =>
-      match Γp with
-      | context[Esnoc _ ?i (@cached P ?c)] =>
-        apply (tac_cached_use i c);
-        [ reflexivity (* lookup should always succeed, found by context match *)
-        | reduction.pm_reduce;
-          reflexivity ]
-      end
-    end.
-
-  (* this is attractively simple but probably doesn't correctly backtrack in
-  iAssumptionCore (for using different caches) *)
-  Ltac iFromCache' :=
-    eapply tac_cached_use;
-    [ iAssumptionCore (* find a cache for the goal *)
-    | cbv [cache_prop cache_names env_to_named_prop env_to_named_prop_go];
-      reduction.pm_reduce;
-      try reflexivity
-    ].
-
-  Declare Scope cache_hide_scope.
-  Notation "'cache_for!' P 'with' Hs" := (@cached _ (Cache P _ Hs)) (at level 29, only printing) : cache_hide_scope.
-  Open Scope cache_hide_scope.
-
   Theorem wpc_RepBlock__Write (Q: iProp Σ) {k E2} γ l k' addr (s: Slice.t) q (b: Block) :
     (S k < k')%nat →
     {{{ "Hrb" ∷ is_rblock γ k' l addr ∗
@@ -360,10 +253,10 @@ Section goose.
     iCache with "HΦ".
     { by crash_case. }
 
-    wpc_pures; first by auto.
+    wpc_pures.
     wpc_bind_seq.
     iApply (use_crash_locked with "His_locked"); auto.
-    iSplit; first by crash_case.
+    iSplit; first by iFromCache.
     iNamed 1.
     iNamed "Hlkinv".
 
@@ -372,9 +265,9 @@ Section goose.
       iExists _; iFrame.
       iExists _; iFrame. }
 
-    wpc_call; first by iFromCache.
+    wpc_call.
     wpc_bind (struct.loadF _ _ _).
-    wpc_frame "HΦ Hprimary Hbackup HP"; first by iFromCache.
+    wpc_frame "HΦ Hprimary Hbackup HP".
     wp_loadField.
     iNamed 1.
     wpc_apply (wpc_Write_fupd (⊤ ∖ ↑N) ("Hprimary" ∷ int.val addr d↦ b ∗
@@ -402,16 +295,16 @@ Section goose.
       iExists _; iFrame.
       iExists _; iFrame. }
 
-    wpc_pures; first by iFromCache.
+    wpc_pures.
     wpc_bind (struct.loadF _ _ _).
-    wpc_frame "HΦ Hprimary Hbackup HP"; first by iFromCache. (* TODO: can we get these from a cache? *)
+    wpc_frame "HΦ Hprimary Hbackup HP". (* TODO: can we get these from a cache? *)
     wp_loadField.
     iNamed 1.
-    wpc_pures; first by iFromCache.
-    wpc_apply (wpc_Write with "[$Hb Hbackup]").
-    { iExists _; iFrame. }
+    wpc_pures.
+    wpc_apply (wpc_Write' with "[$Hb Hbackup]").
+    { iFrame. }
     iSplit; [ | iNext ].
-    { iIntros "Hb". iDeexHyp "Hb".
+    { iIntros "[Hbackup|Hbackup]"; try iFromCache.
       iSplitL "HΦ"; first by crash_case.
       iExists _; iFrame.
       iExists _; iFrame. }
@@ -420,8 +313,8 @@ Section goose.
     { iExists _; iFrame. }
     iIntros "His_locked".
     iSplit; last by iFromCache.
-    wpc_pures; first by crash_case.
-    wpc_frame "HΦ"; first by crash_case.
+    wpc_pures.
+    wpc_frame "HΦ".
     wp_loadField.
     wp_apply (crash_lock.release_spec with "[$His_locked]"); auto.
     iNamed 1.
