src/Helpers/ProofCaching.v
@@ -1,0 +1,182 @@
+From iris.proofmode Require Import tactics environments.
+From Perennial.Helpers Require Import NamedProps.
+
+Section bi.
+  Context {PROP: bi}.
+  Context `{!BiAffine PROP}.
+
+  Record cache (R: PROP) :=
+    Cache { cache_prop :> env PROP;
+            cache_names: list ident; }.
+
+  Arguments cache_names {R} c.
+  Arguments cache_prop {R} c.
+
+  Definition cached_def {R} (c: cache R): PROP :=
+    (□ ([∗] c -∗ R))%I.
+  Definition cached_aux : seal (@cached_def). by eexists. Qed.
+  Definition cached := unseal cached_aux.
+  Definition cached_eq : @cached = @cached_def := seal_eq cached_aux.
+  Arguments cached {R} c.
+
+  Ltac unseal := rewrite cached_eq /cached_def.
+
+  Global Instance cached_Persistent : Persistent (@cached R c).
+  Proof. unseal. apply _. Qed.
+
+  Local Theorem tac_cached_use {Δ: envs PROP} i {R} (c: cache R) :
+    envs_lookup i Δ = Some (true, cached c) →
+    match envs_split base.Left c.(cache_names) Δ with
+    | Some (Γs, _) => Γs.(env_spatial) = c.(cache_prop)
+    | None => False
+    end →
+    envs_entails Δ R.
+  Proof.
+    unseal.
+    iIntros (Hlookup Hsubenv).
+    destruct_with_eqn (envs_split base.Left c.(cache_names) Δ); [ | contradiction ].
+    destruct p as [Γs Γ'].
+    rewrite envs_entails_eq.
+    iIntros "HΔ".
+    iDestruct (envs_lookup_intuitionistic_sound _ _ _ Hlookup with "HΔ") as
+        "[#Hcache HΔ]".
+    iDestruct (envs_split_sound with "HΔ") as "[HΔ1 HΔ2]"; eauto.
+    iDestruct (envs_clear_spatial_sound with "HΔ1") as "(HΔ'&HΔs)".
+    iApply "Hcache".
+    rewrite -Hsubenv.
+    iAssumption.
+  Qed.
+
+  Local Theorem cached_make R (c: cache R) :
+    □ (env_to_named_prop c -∗ R) -∗
+    cached c.
+  Proof.
+    unseal.
+    iIntros "#HR !>".
+    rewrite env_to_named_prop_unname.
+    rewrite env_to_prop_sound.
+    auto.
+  Qed.
+End bi.
+
+Arguments cached {PROP R} c.
+
+Ltac iCache_go P Hs pat :=
+  let Hs := words Hs in
+  let Hs := (eval vm_compute in (INamed <$> Hs)) in
+  let Δ := iGetCtx in
+  let js := reduction.pm_eval (envs_split base.Left Hs Δ) in
+  match js with
+  | Some (?Δ, _) => let Γs := (eval cbv [env_spatial] in Δ.(env_spatial)) in
+                    iAssert (cached (Cache P Γs Hs)) as pat;
+                    [ iApply cached_make; iModIntro;
+                      cbv [env_to_named_prop env_to_named_prop_go cache_prop];
+                      iNamed 1
+                    | ]
+  | None => fail 1 "hypotheses not found"
+  end.
+
+Tactic Notation "iCache" constr(P) "with" constr(Hs) :=
+  iCache_go P Hs "#?".
+
+Ltac iFromCache :=
+  lazymatch goal with
+  | [ |- envs_entails (Envs ?Γp _ _) ?P ] =>
+    first [ match Γp with
+            | context[Esnoc _ ?i (@cached _ P ?c)] =>
+              apply (tac_cached_use i c);
+              [ reflexivity (* lookup should always succeed, found by context match *)
+              | reduction.pm_reduce;
+                reflexivity ]
+            end
+          | lazymatch Γp with
+            | context[Esnoc _ _ (@cached _ P _)] =>
+              fail 1 "iFromCache: could not find hypotheses for any cache"
+            | _ =>
+              fail 1 "iFromCache: no matching caches"
+            end
+          ]
+  end.
+
+Declare Scope cache_hide_scope.
+Notation "'cache_for!' P 'with' Hs" := (cached (Cache P _ Hs))
+                                         (at level 29, only printing) : cache_hide_scope.
+Open Scope cache_hide_scope.
+
+Module examples.
+  Section bi.
+    Context {PROP:bi} `{!BiAffine PROP}.
+    Context (P P1 P2 Q R: PROP).
+    Context (HP: P -∗ P1 ∗ P2).
+    Context (HQ: P1 -∗ Q).
+
+    Example make_and_use_cache :
+      P -∗
+      P1 ∗ (P -∗ P1).
+    Proof.
+      iIntros "HP".
+      iCache P1 with "HP".
+      { iDestruct (HP with "HP") as "[$ _]". }
+      iSplitL "HP".
+      - iFromCache.
+      - iIntros "HP".
+        iFromCache.
+    Qed.
+
+    Example multiple_caches_for_goal :
+      P ∗ Q -∗
+      Q ∗ Q.
+    Proof.
+      iIntros "[HP HQ]".
+      iCache Q with "HP".
+      { iDestruct (HP with "HP") as "[HP1 _]".
+        iDestruct (HQ with "HP1") as "$". }
+      iCache Q with "HQ".
+      { auto. }
+      iSplitL "HP".
+      (* these goals are identical, so one of them requires backtracking on
+      which cache to use *)
+      - iFromCache.
+      - iFromCache.
+    Qed.
+
+    Example reordered_hypotheses :
+      P ∗ Q -∗
+      Q ∗ P.
+    Proof.
+      iIntros "[HP HQ]".
+      iCache (Q ∗ P)%I with "HQ HP".
+      { iFrame. }
+      (* we need to grab the goals from the context in the opposite order that
+      they appear; the current implementation uses envs_split driven by a list
+      of hypotheses in the cache itself to guide the splitting and order *)
+      iFromCache.
+    Qed.
+
+    Example fail_no_hyps :
+      P -∗ P.
+    Proof.
+      iIntros "HP".
+      iCache P with "HP"; first by iFrame.
+      iRename "HP" into "HP'".
+      Fail iFromCache. (* this should report a useful error *)
+    Abort.
+
+    Example fail_wrong_hyps :
+      P ∗ Q -∗ P.
+    Proof.
+      iIntros "[HP HQ]".
+      iCache P with "HP"; first by iFrame.
+      iClear "HP". iRename "HQ" into "HP".
+      Fail iFromCache. (* this should report a useful error *)
+    Abort.
+
+    Example fail_no_cache :
+      P -∗ P.
+    Proof.
+      iIntros "HP".
+      Fail iFromCache. (* this should report a useful error *)
+    Abort.
+
+  End bi.
+End examples.
